src/CodegenCheck/Voblint_OCaml_Check.thy
@@ -22,7 +22,7 @@ export_code
   analyse Sign_Analysis Interval_Analysis
   analyse_ctx Ctx_None Ctx_EntryState
   mk_program proc_decl_of
-  SKIP com.Call Random com.If Assign Seq While Restore Unwind Return Check
+  SKIP com.Call com.If Assign Seq While Restore Unwind Return Check
   N V Plus Minus Times
   Bc bexp.Not And Or Less bexp.Eq
   Check_Proved Check_Refuted Check_Unknown
