src/Examples/Interval/Example_Interval_DG_Flagship.thy
@@ -264,6 +264,7 @@ lemma flagship_wf:
   unfolding wf_compile_input_simps
     flagship_pi_def flagship_prog_def
   by (auto simp: source_aexp_def source_bexp_def proc_decl_of_def ret_var_def reserved_ret_var_def
+      prog_main_name_def special_table_def special_pname_nondet_int_def
       split: if_splits)
 
 theorem flagship_source_run_sound:
