src/Examples/Tooling/Example_State_Report_GraphViz.thy
@@ -319,7 +319,7 @@ export_code
   bexp_vnames_list string_of_abstract_value
   is_bottom_abstract_value program_vars
   mk_program proc_decl_of declared_global_vars pretty_string_of_program
-  SKIP com.Call Random com.If Assign Seq While Restore Unwind Return Check
+  SKIP com.Call com.If Assign Seq While Restore Unwind Return Check
   N V Plus Minus Times
   Bc bexp.Not And Or Less bexp.Eq
   Check_Proved Check_Refuted Check_Unknown
