src/VIMP/VIMP_Source_Print.thy
@@ -60,7 +60,6 @@ fun join_source :: "string \<Rightarrow> string list \<Rightarrow> string" where
 fun string_of_com :: "com \<Rightarrow> string" where
   "string_of_com SKIP = ''skip''"
 | "string_of_com (Assign x e) = String.explode x @ '' := '' @ string_of_aexp e"
-| "string_of_com (Random x) = String.explode x @ '' := random()''"
 | "string_of_com (VIMP_Proc.com.Check c) = ''__voblint_check('' @ string_of_bexp c @ '')''"
 | "string_of_com (Seq c1 c2) =
     string_of_com c1 @ '';'' @ source_nl @ string_of_com c2"
@@ -100,8 +99,6 @@ fun pretty_source_lines_com :: "nat \<Rightarrow> com \<Rightarrow> string list"
   "pretty_source_lines_com n SKIP = [source_indent n @ ''skip'']"
 | "pretty_source_lines_com n (Assign x e) =
     [source_indent n @ String.explode x @ '' := '' @ string_of_aexp e]"
-| "pretty_source_lines_com n (Random x) =
-    [source_indent n @ String.explode x @ '' := random()'']"
 | "pretty_source_lines_com n (VIMP_Proc.com.Check c) =
     [source_indent n @ ''__voblint_check('' @ string_of_bexp c @ '')'']"
 | "pretty_source_lines_com n (Seq c1 c2) =
